proofchat/bin/server/server.ml
@@ -1,9 +1,126 @@
 
 let __ = let rec f _ = Obj.repr f in Obj.repr f
 
+type nat =
+| O
+| S of nat
+
+(** val app : 'a1 list -> 'a1 list -> 'a1 list **)
+
+let app x =
+  let rec app0 l m =
+    match l with
+    | [] -> m
+    | a :: l1 -> a :: (app0 l1 m)
+  in app0 x
+
+type positive =
+| XI of positive
+| XO of positive
+| XH
+
+type n =
+| N0
+| Npos of positive
+
+module Pos =
+ struct
+  (** val succ : positive -> positive **)
+
+  let rec succ = function
+  | XI p -> XO (succ p)
+  | XO p -> XI p
+  | XH -> XO XH
+
+  (** val of_succ_nat : nat -> positive **)
+
+  let rec of_succ_nat = function
+  | O -> XH
+  | S x -> succ (of_succ_nat x)
+ end
+
+module N =
+ struct
+  (** val of_nat : nat -> n **)
+
+  let of_nat = function
+  | O -> N0
+  | S n' -> Npos (Pos.of_succ_nat n')
+ end
+
+(** val zero : char **)
+
+let zero = '\000'
+
+(** val one : char **)
+
+let one = '\001'
+
+(** val shift : bool -> char -> char **)
+
+let shift = fun b c -> Char.chr (((Char.code c) lsl 1) land 255 + if b then 1 else 0)
+
+(** val ascii_of_pos : positive -> char **)
+
+let ascii_of_pos =
+  let rec loop n0 p =
+    match n0 with
+    | O -> zero
+    | S n' ->
+      (match p with
+       | XI p' -> shift true (loop n' p')
+       | XO p' -> shift false (loop n' p')
+       | XH -> one)
+  in loop (S (S (S (S (S (S (S (S O))))))))
+
+(** val ascii_of_N : n -> char **)
+
+let ascii_of_N = function
+| N0 -> zero
+| Npos p -> ascii_of_pos p
+
+(** val ascii_of_nat : nat -> char **)
+
+let ascii_of_nat a =
+  ascii_of_N (N.of_nat a)
+
+
+
+(** val rev : 'a1 list -> 'a1 list **)
+
+let rev l =
+  let rec rev0 = function
+  | [] -> []
+  | x :: l' -> app (rev0 l') (x :: [])
+  in rev0 l
+
+(** val concat : 'a1 list list -> 'a1 list **)
+
+let concat l =
+  let rec concat0 = function
+  | [] -> []
+  | x :: l1 -> app x (concat0 l1)
+  in concat0 l
+
+(** val map : ('a1 -> 'a2) -> 'a1 list -> 'a2 list **)
+
+let map f =
+  let rec map0 = function
+  | [] -> []
+  | a :: t -> (f a) :: (map0 t)
+  in map0
+
+(** val add : Uint63.t -> Uint63.t -> Uint63.t **)
+
+let add = Uint63.add
+
 (** val sub : Uint63.t -> Uint63.t -> Uint63.t **)
 
 let sub = Uint63.sub
+
+(** val eqb : Uint63.t -> Uint63.t -> bool **)
+
+let eqb = Uint63.equal
 
 (** val ltsb : Uint63.t -> Uint63.t -> bool **)
 
@@ -22,25 +139,67 @@ type 'x optionE =
 | SomeE of 'x
 | NoneE of string
 
+type bytes = char list
+
+(** val send :
+    Unix.file_descr -> bytes -> Uint63.t -> Uint63.t -> Unix.msg_flag list ->
+    Uint63.t **)
+
+let send = (fun a b c d e -> Unix.send a (Proofchat.Pfbytes.bytes_of_char_list b) c d e)
+
+(** val recv :
+    Unix.file_descr -> Uint63.t -> Uint63.t -> Unix.msg_flag list ->
+    Uint63.t * bytes **)
+
+let recv = Proofchat.Pfbytes.functional_read
+
+(** val keep : 'a1 -> unit **)
+
+let keep = (fun _ -> ())
+
 (** val sub1_no_underflow : Uint63.t -> bool **)
 
-let sub1_no_underflow n =
-  (&&) (lesb (Uint63.of_int (0)) (sub n (Uint63.of_int (1))))
-    (ltsb (sub n (Uint63.of_int (1))) n)
+let sub1_no_underflow n0 =
+  (&&) (lesb (Uint63.of_int (0)) (sub n0 (Uint63.of_int (1))))
+    (ltsb (sub n0 (Uint63.of_int (1))) n0)
+
+type repeat_until_timeout_code =
+| Recurse
+| EarlyStopSuccess
+| EarlyStopFailure of string
 
 (** val repeat_until_timeout :
-    Uint63.t -> (unit -> unit optionE) -> unit optionE **)
+    Uint63.t -> (unit -> repeat_until_timeout_code) -> unit optionE **)
 
 let repeat_until_timeout x x0 =
   let rec hrec timeout f _ =
     (if sub1_no_underflow timeout
      then (fun _ ->
             (match f () with
-             | SomeE x1 -> (fun _ -> SomeE x1)
-             | NoneE _ ->
-               (fun _ -> hrec (sub timeout (Uint63.of_int (1))) f __)) __)
+             | Recurse ->
+               (fun _ -> hrec (sub timeout (Uint63.of_int (1))) f __)
+             | EarlyStopSuccess -> (fun _ -> SomeE ())
+             | EarlyStopFailure s -> (fun _ -> NoneE s)) __)
      else (fun _ -> NoneE "Timeout occurred")) __
   in hrec x x0 __
+
+(** val space : char **)
+
+let space =
+  ascii_of_nat (S (S (S (S (S (S (S (S (S (S (S (S (S (S (S (S (S (S (S (S (S
+    (S (S (S (S (S (S (S (S (S (S (S O))))))))))))))))))))))))))))))))
+
+(** val no_spaces : string -> bool **)
+
+let rec no_spaces s =
+  (* If this appears, you're using String internals. Please don't *)
+ (fun f0 f1 s ->
+    let l = String.length s in
+    if l = 0 then f0 () else f1 (String.get s 0) (String.sub s 1 (l-1)))
+
+    (fun _ -> true)
+    (fun a s' -> if (=) a space then false else no_spaces s')
+    s
 
 (** val string_of_socket_addr : Unix.sockaddr -> string **)
 
@@ -49,6 +208,770 @@ let string_of_socket_addr = function
 | Unix.ADDR_INET (addr, p) ->
   (^) (Unix.string_of_inet_addr addr) ((^) ":" (string_of_int p))
 
+(** val int_len_list : 'a1 list -> Uint63.t **)
+
+let rec int_len_list = function
+| [] -> (Uint63.of_int (0))
+| _ :: t -> add (Uint63.of_int (1)) (int_len_list t)
+
+(** val bytes_of_string : string -> bytes **)
+
+let rec bytes_of_string s =
+  (* If this appears, you're using String internals. Please don't *)
+ (fun f0 f1 s ->
+    let l = String.length s in
+    if l = 0 then f0 () else f1 (String.get s 0) (String.sub s 1 (l-1)))
+
+    (fun _ -> [])
+    (fun a s' -> ((fun x -> x) a) :: (bytes_of_string s'))
+    s
+
+(** val string_of_bytes : bytes -> string **)
+
+let rec string_of_bytes = function
+| [] -> ""
+| h :: t ->
+  (* If this appears, you're using String internals. Please don't *)
+  (fun (c, s) -> String.make 1 c ^ s)
+
+    (((fun x -> x) h), (string_of_bytes t))
+
+(** val int_len_string : string -> Uint63.t **)
+
+let int_len_string s =
+  int_len_list (bytes_of_string s)
+
+(** val create_list : 'a1 -> Uint63.t -> 'a1 list **)
+
+let create_list x0 x1 =
+  let rec hrec _ x n0 _ =
+    (if sub1_no_underflow n0
+     then (fun _ -> x :: (hrec __ x (sub n0 (Uint63.of_int (1))) __))
+     else (fun _ -> [])) __
+  in hrec __ x0 x1 __
+
+(** val pad_string_r : string -> char -> Uint63.t -> string **)
+
+let pad_string_r s b target_len =
+  (^) s (string_of_bytes (create_list b (sub target_len (int_len_string s))))
+
+(** val first_n : 'a1 list -> Uint63.t -> 'a1 list optionE **)
+
+let rec first_n l n0 =
+  match l with
+  | [] ->
+    if eqb n0 (Uint63.of_int (0)) then SomeE [] else NoneE "first_n failure"
+  | h :: t ->
+    if lesb (Uint63.of_int (1)) n0
+    then (match first_n t (sub n0 (Uint63.of_int (1))) with
+          | SomeE rec_answer -> SomeE (h :: rec_answer)
+          | NoneE err -> NoneE err)
+    else SomeE []
+
+(** val last_n : 'a1 list -> Uint63.t -> 'a1 list optionE **)
+
+let last_n l n0 =
+  match first_n (rev l) n0 with
+  | SomeE aux -> SomeE (rev aux)
+  | NoneE err -> NoneE err
+
+type username =
+  string
+  (* singleton inductive, whose constructor was Build_username *)
+
+(** val validate_username : string -> bool **)
+
+let validate_username name =
+  (&&)
+    ((&&) (lesb (Uint63.of_int (1)) (int_len_string name))
+      (lesb (int_len_string name) (Uint63.of_int (32)))) (no_spaces name)
+
+(** val new_username : string -> username optionE **)
+
+let new_username s =
+  let b = validate_username s in
+  (if b
+   then (fun _ -> SomeE s)
+   else (fun _ ->
+          let b0 = no_spaces s in
+          if b0
+          then NoneE "Username length must be in range [1..32]"
+          else NoneE "Username cannot contain spaces")) __
+
+(** val dummy_username : username **)
+
+let dummy_username =
+  "X"
+
+(** val serialize_string : string -> bytes **)
+
+let serialize_string s =
+  app (Proofchat.Pfbytes.int63_to_bytes (int_len_string s))
+    (bytes_of_string s)
+
+(** val serialize_username : username -> bytes **)
+
+let serialize_username u =
+  bytes_of_string (pad_string_r u '\x00' (Uint63.of_int (32)))
+
+type client_message =
+| REG of username
+| MESG of string
+| PMSG of string * username
+| EXIT of username
+
+(** val deserialize_client_message : bytes -> client_message optionE **)
+
+let deserialize_client_message b = match b with
+| [] -> NoneE ((^) "Client message code not recognized: " (string_of_bytes b))
+| b0 :: t ->
+  (match b0 with
+   | '\x00' ->
+     (match new_username (string_of_bytes t) with
+      | SomeE uname -> SomeE (REG uname)
+      | NoneE err -> NoneE err)
+   | '\x01' -> SomeE (MESG (string_of_bytes t))
+   | '\x02' ->
+     (match first_n t (Uint63.of_int (32)) with
+      | SomeE name_bytes ->
+        (match new_username (string_of_bytes name_bytes) with
+         | SomeE uname ->
+           (match last_n t (sub (int_len_list t) (Uint63.of_int (32))) with
+            | SomeE msg_bytes ->
+              SomeE (PMSG ((string_of_bytes msg_bytes), uname))
+            | NoneE err -> NoneE err)
+         | NoneE err -> NoneE err)
+      | NoneE err -> NoneE err)
+   | '\x03' ->
+     (match new_username (string_of_bytes t) with
+      | SomeE uname -> SomeE (EXIT uname)
+      | NoneE err -> NoneE err)
+   | '\x04' ->
+     NoneE ((^) "Client message code not recognized: " (string_of_bytes b))
+   | '\x05' ->
+     NoneE ((^) "Client message code not recognized: " (string_of_bytes b))
+   | '\x06' ->
+     NoneE ((^) "Client message code not recognized: " (string_of_bytes b))
+   | '\x07' ->
+     NoneE ((^) "Client message code not recognized: " (string_of_bytes b))
+   | '\x08' ->
+     NoneE ((^) "Client message code not recognized: " (string_of_bytes b))
+   | '\t' ->
+     NoneE ((^) "Client message code not recognized: " (string_of_bytes b))
+   | '\n' ->
+     NoneE ((^) "Client message code not recognized: " (string_of_bytes b))
+   | '\x0b' ->
+     NoneE ((^) "Client message code not recognized: " (string_of_bytes b))
+   | '\x0c' ->
+     NoneE ((^) "Client message code not recognized: " (string_of_bytes b))
+   | '\r' ->
+     NoneE ((^) "Client message code not recognized: " (string_of_bytes b))
+   | '\x0e' ->
+     NoneE ((^) "Client message code not recognized: " (string_of_bytes b))
+   | '\x0f' ->
+     NoneE ((^) "Client message code not recognized: " (string_of_bytes b))
+   | '\x10' ->
+     NoneE ((^) "Client message code not recognized: " (string_of_bytes b))
+   | '\x11' ->
+     NoneE ((^) "Client message code not recognized: " (string_of_bytes b))
+   | '\x12' ->
+     NoneE ((^) "Client message code not recognized: " (string_of_bytes b))
+   | '\x13' ->
+     NoneE ((^) "Client message code not recognized: " (string_of_bytes b))
+   | '\x14' ->
+     NoneE ((^) "Client message code not recognized: " (string_of_bytes b))
+   | '\x15' ->
+     NoneE ((^) "Client message code not recognized: " (string_of_bytes b))
+   | '\x16' ->
+     NoneE ((^) "Client message code not recognized: " (string_of_bytes b))
+   | '\x17' ->
+     NoneE ((^) "Client message code not recognized: " (string_of_bytes b))
+   | '\x18' ->
+     NoneE ((^) "Client message code not recognized: " (string_of_bytes b))
+   | '\x19' ->
+     NoneE ((^) "Client message code not recognized: " (string_of_bytes b))
+   | '\x1a' ->
+     NoneE ((^) "Client message code not recognized: " (string_of_bytes b))
+   | '\x1b' ->
+     NoneE ((^) "Client message code not recognized: " (string_of_bytes b))
+   | '\x1c' ->
+     NoneE ((^) "Client message code not recognized: " (string_of_bytes b))
+   | '\x1d' ->
+     NoneE ((^) "Client message code not recognized: " (string_of_bytes b))
+   | '\x1e' ->
+     NoneE ((^) "Client message code not recognized: " (string_of_bytes b))
+   | '\x1f' ->
+     NoneE ((^) "Client message code not recognized: " (string_of_bytes b))
+   | ' ' ->
+     NoneE ((^) "Client message code not recognized: " (string_of_bytes b))
+   | '!' ->
+     NoneE ((^) "Client message code not recognized: " (string_of_bytes b))
+   | '"' ->
+     NoneE ((^) "Client message code not recognized: " (string_of_bytes b))
+   | '#' ->
+     NoneE ((^) "Client message code not recognized: " (string_of_bytes b))
+   | '$' ->
+     NoneE ((^) "Client message code not recognized: " (string_of_bytes b))
+   | '%' ->
+     NoneE ((^) "Client message code not recognized: " (string_of_bytes b))
+   | '&' ->
+     NoneE ((^) "Client message code not recognized: " (string_of_bytes b))
+   | '\'' ->
+     NoneE ((^) "Client message code not recognized: " (string_of_bytes b))
+   | '(' ->
+     NoneE ((^) "Client message code not recognized: " (string_of_bytes b))
+   | ')' ->
+     NoneE ((^) "Client message code not recognized: " (string_of_bytes b))
+   | '*' ->
+     NoneE ((^) "Client message code not recognized: " (string_of_bytes b))
+   | '+' ->
+     NoneE ((^) "Client message code not recognized: " (string_of_bytes b))
+   | ',' ->
+     NoneE ((^) "Client message code not recognized: " (string_of_bytes b))
+   | '-' ->
+     NoneE ((^) "Client message code not recognized: " (string_of_bytes b))
+   | '.' ->
+     NoneE ((^) "Client message code not recognized: " (string_of_bytes b))
+   | '/' ->
+     NoneE ((^) "Client message code not recognized: " (string_of_bytes b))
+   | '0' ->
+     NoneE ((^) "Client message code not recognized: " (string_of_bytes b))
+   | '1' ->
+     NoneE ((^) "Client message code not recognized: " (string_of_bytes b))
+   | '2' ->
+     NoneE ((^) "Client message code not recognized: " (string_of_bytes b))
+   | '3' ->
+     NoneE ((^) "Client message code not recognized: " (string_of_bytes b))
+   | '4' ->
+     NoneE ((^) "Client message code not recognized: " (string_of_bytes b))
+   | '5' ->
+     NoneE ((^) "Client message code not recognized: " (string_of_bytes b))
+   | '6' ->
+     NoneE ((^) "Client message code not recognized: " (string_of_bytes b))
+   | '7' ->
+     NoneE ((^) "Client message code not recognized: " (string_of_bytes b))
+   | '8' ->
+     NoneE ((^) "Client message code not recognized: " (string_of_bytes b))
+   | '9' ->
+     NoneE ((^) "Client message code not recognized: " (string_of_bytes b))
+   | ':' ->
+     NoneE ((^) "Client message code not recognized: " (string_of_bytes b))
+   | ';' ->
+     NoneE ((^) "Client message code not recognized: " (string_of_bytes b))
+   | '<' ->
+     NoneE ((^) "Client message code not recognized: " (string_of_bytes b))
+   | '=' ->
+     NoneE ((^) "Client message code not recognized: " (string_of_bytes b))
+   | '>' ->
+     NoneE ((^) "Client message code not recognized: " (string_of_bytes b))
+   | '?' ->
+     NoneE ((^) "Client message code not recognized: " (string_of_bytes b))
+   | '@' ->
+     NoneE ((^) "Client message code not recognized: " (string_of_bytes b))
+   | 'A' ->
+     NoneE ((^) "Client message code not recognized: " (string_of_bytes b))
+   | 'B' ->
+     NoneE ((^) "Client message code not recognized: " (string_of_bytes b))
+   | 'C' ->
+     NoneE ((^) "Client message code not recognized: " (string_of_bytes b))
+   | 'D' ->
+     NoneE ((^) "Client message code not recognized: " (string_of_bytes b))
+   | 'E' ->
+     NoneE ((^) "Client message code not recognized: " (string_of_bytes b))
+   | 'F' ->
+     NoneE ((^) "Client message code not recognized: " (string_of_bytes b))
+   | 'G' ->
+     NoneE ((^) "Client message code not recognized: " (string_of_bytes b))
+   | 'H' ->
+     NoneE ((^) "Client message code not recognized: " (string_of_bytes b))
+   | 'I' ->
+     NoneE ((^) "Client message code not recognized: " (string_of_bytes b))
+   | 'J' ->
+     NoneE ((^) "Client message code not recognized: " (string_of_bytes b))
+   | 'K' ->
+     NoneE ((^) "Client message code not recognized: " (string_of_bytes b))
+   | 'L' ->
+     NoneE ((^) "Client message code not recognized: " (string_of_bytes b))
+   | 'M' ->
+     NoneE ((^) "Client message code not recognized: " (string_of_bytes b))
+   | 'N' ->
+     NoneE ((^) "Client message code not recognized: " (string_of_bytes b))
+   | 'O' ->
+     NoneE ((^) "Client message code not recognized: " (string_of_bytes b))
+   | 'P' ->
+     NoneE ((^) "Client message code not recognized: " (string_of_bytes b))
+   | 'Q' ->
+     NoneE ((^) "Client message code not recognized: " (string_of_bytes b))
+   | 'R' ->
+     NoneE ((^) "Client message code not recognized: " (string_of_bytes b))
+   | 'S' ->
+     NoneE ((^) "Client message code not recognized: " (string_of_bytes b))
+   | 'T' ->
+     NoneE ((^) "Client message code not recognized: " (string_of_bytes b))
+   | 'U' ->
+     NoneE ((^) "Client message code not recognized: " (string_of_bytes b))
+   | 'V' ->
+     NoneE ((^) "Client message code not recognized: " (string_of_bytes b))
+   | 'W' ->
+     NoneE ((^) "Client message code not recognized: " (string_of_bytes b))
+   | 'X' ->
+     NoneE ((^) "Client message code not recognized: " (string_of_bytes b))
+   | 'Y' ->
+     NoneE ((^) "Client message code not recognized: " (string_of_bytes b))
+   | 'Z' ->
+     NoneE ((^) "Client message code not recognized: " (string_of_bytes b))
+   | '[' ->
+     NoneE ((^) "Client message code not recognized: " (string_of_bytes b))
+   | '\\' ->
+     NoneE ((^) "Client message code not recognized: " (string_of_bytes b))
+   | ']' ->
+     NoneE ((^) "Client message code not recognized: " (string_of_bytes b))
+   | '^' ->
+     NoneE ((^) "Client message code not recognized: " (string_of_bytes b))
+   | '_' ->
+     NoneE ((^) "Client message code not recognized: " (string_of_bytes b))
+   | '`' ->
+     NoneE ((^) "Client message code not recognized: " (string_of_bytes b))
+   | 'a' ->
+     NoneE ((^) "Client message code not recognized: " (string_of_bytes b))
+   | 'b' ->
+     NoneE ((^) "Client message code not recognized: " (string_of_bytes b))
+   | 'c' ->
+     NoneE ((^) "Client message code not recognized: " (string_of_bytes b))
+   | 'd' ->
+     NoneE ((^) "Client message code not recognized: " (string_of_bytes b))
+   | 'e' ->
+     NoneE ((^) "Client message code not recognized: " (string_of_bytes b))
+   | 'f' ->
+     NoneE ((^) "Client message code not recognized: " (string_of_bytes b))
+   | 'g' ->
+     NoneE ((^) "Client message code not recognized: " (string_of_bytes b))
+   | 'h' ->
+     NoneE ((^) "Client message code not recognized: " (string_of_bytes b))
+   | 'i' ->
+     NoneE ((^) "Client message code not recognized: " (string_of_bytes b))
+   | 'j' ->
+     NoneE ((^) "Client message code not recognized: " (string_of_bytes b))
+   | 'k' ->
+     NoneE ((^) "Client message code not recognized: " (string_of_bytes b))
+   | 'l' ->
+     NoneE ((^) "Client message code not recognized: " (string_of_bytes b))
+   | 'm' ->
+     NoneE ((^) "Client message code not recognized: " (string_of_bytes b))
+   | 'n' ->
+     NoneE ((^) "Client message code not recognized: " (string_of_bytes b))
+   | 'o' ->
+     NoneE ((^) "Client message code not recognized: " (string_of_bytes b))
+   | 'p' ->
+     NoneE ((^) "Client message code not recognized: " (string_of_bytes b))
+   | 'q' ->
+     NoneE ((^) "Client message code not recognized: " (string_of_bytes b))
+   | 'r' ->
+     NoneE ((^) "Client message code not recognized: " (string_of_bytes b))
+   | 's' ->
+     NoneE ((^) "Client message code not recognized: " (string_of_bytes b))
+   | 't' ->
+     NoneE ((^) "Client message code not recognized: " (string_of_bytes b))
+   | 'u' ->
+     NoneE ((^) "Client message code not recognized: " (string_of_bytes b))
+   | 'v' ->
+     NoneE ((^) "Client message code not recognized: " (string_of_bytes b))
+   | 'w' ->
+     NoneE ((^) "Client message code not recognized: " (string_of_bytes b))
+   | 'x' ->
+     NoneE ((^) "Client message code not recognized: " (string_of_bytes b))
+   | 'y' ->
+     NoneE ((^) "Client message code not recognized: " (string_of_bytes b))
+   | 'z' ->
+     NoneE ((^) "Client message code not recognized: " (string_of_bytes b))
+   | '{' ->
+     NoneE ((^) "Client message code not recognized: " (string_of_bytes b))
+   | '|' ->
+     NoneE ((^) "Client message code not recognized: " (string_of_bytes b))
+   | '}' ->
+     NoneE ((^) "Client message code not recognized: " (string_of_bytes b))
+   | '~' ->
+     NoneE ((^) "Client message code not recognized: " (string_of_bytes b))
+   | '\x7f' ->
+     NoneE ((^) "Client message code not recognized: " (string_of_bytes b))
+   | '\x80' ->
+     NoneE ((^) "Client message code not recognized: " (string_of_bytes b))
+   | '\x81' ->
+     NoneE ((^) "Client message code not recognized: " (string_of_bytes b))
+   | '\x82' ->
+     NoneE ((^) "Client message code not recognized: " (string_of_bytes b))
+   | '\x83' ->
+     NoneE ((^) "Client message code not recognized: " (string_of_bytes b))
+   | '\x84' ->
+     NoneE ((^) "Client message code not recognized: " (string_of_bytes b))
+   | '\x85' ->
+     NoneE ((^) "Client message code not recognized: " (string_of_bytes b))
+   | '\x86' ->
+     NoneE ((^) "Client message code not recognized: " (string_of_bytes b))
+   | '\x87' ->
+     NoneE ((^) "Client message code not recognized: " (string_of_bytes b))
+   | '\x88' ->
+     NoneE ((^) "Client message code not recognized: " (string_of_bytes b))
+   | '\x89' ->
+     NoneE ((^) "Client message code not recognized: " (string_of_bytes b))
+   | '\x8a' ->
+     NoneE ((^) "Client message code not recognized: " (string_of_bytes b))
+   | '\x8b' ->
+     NoneE ((^) "Client message code not recognized: " (string_of_bytes b))
+   | '\x8c' ->
+     NoneE ((^) "Client message code not recognized: " (string_of_bytes b))
+   | '\x8d' ->
+     NoneE ((^) "Client message code not recognized: " (string_of_bytes b))
+   | '\x8e' ->
+     NoneE ((^) "Client message code not recognized: " (string_of_bytes b))
+   | '\x8f' ->
+     NoneE ((^) "Client message code not recognized: " (string_of_bytes b))
+   | '\x90' ->
+     NoneE ((^) "Client message code not recognized: " (string_of_bytes b))
+   | '\x91' ->
+     NoneE ((^) "Client message code not recognized: " (string_of_bytes b))
+   | '\x92' ->
+     NoneE ((^) "Client message code not recognized: " (string_of_bytes b))
+   | '\x93' ->
+     NoneE ((^) "Client message code not recognized: " (string_of_bytes b))
+   | '\x94' ->
+     NoneE ((^) "Client message code not recognized: " (string_of_bytes b))
+   | '\x95' ->
+     NoneE ((^) "Client message code not recognized: " (string_of_bytes b))
+   | '\x96' ->
+     NoneE ((^) "Client message code not recognized: " (string_of_bytes b))
+   | '\x97' ->
+     NoneE ((^) "Client message code not recognized: " (string_of_bytes b))
+   | '\x98' ->
+     NoneE ((^) "Client message code not recognized: " (string_of_bytes b))
+   | '\x99' ->
+     NoneE ((^) "Client message code not recognized: " (string_of_bytes b))
+   | '\x9a' ->
+     NoneE ((^) "Client message code not recognized: " (string_of_bytes b))
+   | '\x9b' ->
+     NoneE ((^) "Client message code not recognized: " (string_of_bytes b))
+   | '\x9c' ->
+     NoneE ((^) "Client message code not recognized: " (string_of_bytes b))
+   | '\x9d' ->
+     NoneE ((^) "Client message code not recognized: " (string_of_bytes b))
+   | '\x9e' ->
+     NoneE ((^) "Client message code not recognized: " (string_of_bytes b))
+   | '\x9f' ->
+     NoneE ((^) "Client message code not recognized: " (string_of_bytes b))
+   | '\xa0' ->
+     NoneE ((^) "Client message code not recognized: " (string_of_bytes b))
+   | '\xa1' ->
+     NoneE ((^) "Client message code not recognized: " (string_of_bytes b))
+   | '\xa2' ->
+     NoneE ((^) "Client message code not recognized: " (string_of_bytes b))
+   | '\xa3' ->
+     NoneE ((^) "Client message code not recognized: " (string_of_bytes b))
+   | '\xa4' ->
+     NoneE ((^) "Client message code not recognized: " (string_of_bytes b))
+   | '\xa5' ->
+     NoneE ((^) "Client message code not recognized: " (string_of_bytes b))
+   | '\xa6' ->
+     NoneE ((^) "Client message code not recognized: " (string_of_bytes b))
+   | '\xa7' ->
+     NoneE ((^) "Client message code not recognized: " (string_of_bytes b))
+   | '\xa8' ->
+     NoneE ((^) "Client message code not recognized: " (string_of_bytes b))
+   | '\xa9' ->
+     NoneE ((^) "Client message code not recognized: " (string_of_bytes b))
+   | '\xaa' ->
+     NoneE ((^) "Client message code not recognized: " (string_of_bytes b))
+   | '\xab' ->
+     NoneE ((^) "Client message code not recognized: " (string_of_bytes b))
+   | '\xac' ->
+     NoneE ((^) "Client message code not recognized: " (string_of_bytes b))
+   | '\xad' ->
+     NoneE ((^) "Client message code not recognized: " (string_of_bytes b))
+   | '\xae' ->
+     NoneE ((^) "Client message code not recognized: " (string_of_bytes b))
+   | '\xaf' ->
+     NoneE ((^) "Client message code not recognized: " (string_of_bytes b))
+   | '\xb0' ->
+     NoneE ((^) "Client message code not recognized: " (string_of_bytes b))
+   | '\xb1' ->
+     NoneE ((^) "Client message code not recognized: " (string_of_bytes b))
+   | '\xb2' ->
+     NoneE ((^) "Client message code not recognized: " (string_of_bytes b))
+   | '\xb3' ->
+     NoneE ((^) "Client message code not recognized: " (string_of_bytes b))
+   | '\xb4' ->
+     NoneE ((^) "Client message code not recognized: " (string_of_bytes b))
+   | '\xb5' ->
+     NoneE ((^) "Client message code not recognized: " (string_of_bytes b))
+   | '\xb6' ->
+     NoneE ((^) "Client message code not recognized: " (string_of_bytes b))
+   | '\xb7' ->
+     NoneE ((^) "Client message code not recognized: " (string_of_bytes b))
+   | '\xb8' ->
+     NoneE ((^) "Client message code not recognized: " (string_of_bytes b))
+   | '\xb9' ->
+     NoneE ((^) "Client message code not recognized: " (string_of_bytes b))
+   | '\xba' ->
+     NoneE ((^) "Client message code not recognized: " (string_of_bytes b))
+   | '\xbb' ->
+     NoneE ((^) "Client message code not recognized: " (string_of_bytes b))
+   | '\xbc' ->
+     NoneE ((^) "Client message code not recognized: " (string_of_bytes b))
+   | '\xbd' ->
+     NoneE ((^) "Client message code not recognized: " (string_of_bytes b))
+   | '\xbe' ->
+     NoneE ((^) "Client message code not recognized: " (string_of_bytes b))
+   | '\xbf' ->
+     NoneE ((^) "Client message code not recognized: " (string_of_bytes b))
+   | '\xc0' ->
+     NoneE ((^) "Client message code not recognized: " (string_of_bytes b))
+   | '\xc1' ->
+     NoneE ((^) "Client message code not recognized: " (string_of_bytes b))
+   | '\xc2' ->
+     NoneE ((^) "Client message code not recognized: " (string_of_bytes b))
+   | '\xc3' ->
+     NoneE ((^) "Client message code not recognized: " (string_of_bytes b))
+   | '\xc4' ->
+     NoneE ((^) "Client message code not recognized: " (string_of_bytes b))
+   | '\xc5' ->
+     NoneE ((^) "Client message code not recognized: " (string_of_bytes b))
+   | '\xc6' ->
+     NoneE ((^) "Client message code not recognized: " (string_of_bytes b))
+   | '\xc7' ->
+     NoneE ((^) "Client message code not recognized: " (string_of_bytes b))
+   | '\xc8' ->
+     NoneE ((^) "Client message code not recognized: " (string_of_bytes b))
+   | '\xc9' ->
+     NoneE ((^) "Client message code not recognized: " (string_of_bytes b))
+   | '\xca' ->
+     NoneE ((^) "Client message code not recognized: " (string_of_bytes b))
+   | '\xcb' ->
+     NoneE ((^) "Client message code not recognized: " (string_of_bytes b))
+   | '\xcc' ->
+     NoneE ((^) "Client message code not recognized: " (string_of_bytes b))
+   | '\xcd' ->
+     NoneE ((^) "Client message code not recognized: " (string_of_bytes b))
+   | '\xce' ->
+     NoneE ((^) "Client message code not recognized: " (string_of_bytes b))
+   | '\xcf' ->
+     NoneE ((^) "Client message code not recognized: " (string_of_bytes b))
+   | '\xd0' ->
+     NoneE ((^) "Client message code not recognized: " (string_of_bytes b))
+   | '\xd1' ->
+     NoneE ((^) "Client message code not recognized: " (string_of_bytes b))
+   | '\xd2' ->
+     NoneE ((^) "Client message code not recognized: " (string_of_bytes b))
+   | '\xd3' ->
+     NoneE ((^) "Client message code not recognized: " (string_of_bytes b))
+   | '\xd4' ->
+     NoneE ((^) "Client message code not recognized: " (string_of_bytes b))
+   | '\xd5' ->
+     NoneE ((^) "Client message code not recognized: " (string_of_bytes b))
+   | '\xd6' ->
+     NoneE ((^) "Client message code not recognized: " (string_of_bytes b))
+   | '\xd7' ->
+     NoneE ((^) "Client message code not recognized: " (string_of_bytes b))
+   | '\xd8' ->
+     NoneE ((^) "Client message code not recognized: " (string_of_bytes b))
+   | '\xd9' ->
+     NoneE ((^) "Client message code not recognized: " (string_of_bytes b))
+   | '\xda' ->
+     NoneE ((^) "Client message code not recognized: " (string_of_bytes b))
+   | '\xdb' ->
+     NoneE ((^) "Client message code not recognized: " (string_of_bytes b))
+   | '\xdc' ->
+     NoneE ((^) "Client message code not recognized: " (string_of_bytes b))
+   | '\xdd' ->
+     NoneE ((^) "Client message code not recognized: " (string_of_bytes b))
+   | '\xde' ->
+     NoneE ((^) "Client message code not recognized: " (string_of_bytes b))
+   | '\xdf' ->
+     NoneE ((^) "Client message code not recognized: " (string_of_bytes b))
+   | '\xe0' ->
+     NoneE ((^) "Client message code not recognized: " (string_of_bytes b))
+   | '\xe1' ->
+     NoneE ((^) "Client message code not recognized: " (string_of_bytes b))
+   | '\xe2' ->
+     NoneE ((^) "Client message code not recognized: " (string_of_bytes b))
+   | '\xe3' ->
+     NoneE ((^) "Client message code not recognized: " (string_of_bytes b))
+   | '\xe4' ->
+     NoneE ((^) "Client message code not recognized: " (string_of_bytes b))
+   | '\xe5' ->
+     NoneE ((^) "Client message code not recognized: " (string_of_bytes b))
+   | '\xe6' ->
+     NoneE ((^) "Client message code not recognized: " (string_of_bytes b))
+   | '\xe7' ->
+     NoneE ((^) "Client message code not recognized: " (string_of_bytes b))
+   | '\xe8' ->
+     NoneE ((^) "Client message code not recognized: " (string_of_bytes b))
+   | '\xe9' ->
+     NoneE ((^) "Client message code not recognized: " (string_of_bytes b))
+   | '\xea' ->
+     NoneE ((^) "Client message code not recognized: " (string_of_bytes b))
+   | '\xeb' ->
+     NoneE ((^) "Client message code not recognized: " (string_of_bytes b))
+   | '\xec' ->
+     NoneE ((^) "Client message code not recognized: " (string_of_bytes b))
+   | '\xed' ->
+     NoneE ((^) "Client message code not recognized: " (string_of_bytes b))
+   | '\xee' ->
+     NoneE ((^) "Client message code not recognized: " (string_of_bytes b))
+   | '\xef' ->
+     NoneE ((^) "Client message code not recognized: " (string_of_bytes b))
+   | '\xf0' ->
+     NoneE ((^) "Client message code not recognized: " (string_of_bytes b))
+   | '\xf1' ->
+     NoneE ((^) "Client message code not recognized: " (string_of_bytes b))
+   | '\xf2' ->
+     NoneE ((^) "Client message code not recognized: " (string_of_bytes b))
+   | '\xf3' ->
+     NoneE ((^) "Client message code not recognized: " (string_of_bytes b))
+   | '\xf4' ->
+     NoneE ((^) "Client message code not recognized: " (string_of_bytes b))
+   | '\xf5' ->
+     NoneE ((^) "Client message code not recognized: " (string_of_bytes b))
+   | '\xf6' ->
+     NoneE ((^) "Client message code not recognized: " (string_of_bytes b))
+   | '\xf7' ->
+     NoneE ((^) "Client message code not recognized: " (string_of_bytes b))
+   | '\xf8' ->
+     NoneE ((^) "Client message code not recognized: " (string_of_bytes b))
+   | '\xf9' ->
+     NoneE ((^) "Client message code not recognized: " (string_of_bytes b))
+   | '\xfa' ->
+     NoneE ((^) "Client message code not recognized: " (string_of_bytes b))
+   | '\xfb' ->
+     NoneE ((^) "Client message code not recognized: " (string_of_bytes b))
+   | '\xfc' ->
+     NoneE ((^) "Client message code not recognized: " (string_of_bytes b))
+   | '\xfd' ->
+     NoneE ((^) "Client message code not recognized: " (string_of_bytes b))
+   | '\xfe' ->
+     NoneE ((^) "Client message code not recognized: " (string_of_bytes b))
+   | '\xff' ->
+     NoneE ((^) "Client message code not recognized: " (string_of_bytes b)))
+
+type error =
+| UsernameTaken
+| UsernameTooLong
+| UsernameHasSpaces
+| PmsgTargetNotExists
+| UnknownMessageFormat
+| Error
+
+(** val int_of_error : error -> Uint63.t **)
+
+let int_of_error = function
+| UsernameTaken -> (Uint63.of_int (0))
+| UsernameTooLong -> (Uint63.of_int (1))
+| UsernameHasSpaces -> (Uint63.of_int (2))
+| PmsgTargetNotExists -> (Uint63.of_int (3))
+| UnknownMessageFormat -> (Uint63.of_int (4))
+| Error -> (Uint63.of_int (5))
+
+type server_message =
+| ACK of Uint63.t * username list
+| MSG of username * string
+| ERR of error
+
+(** val serialize_server_message : server_message -> bytes **)
+
+let serialize_server_message = function
+| ACK (num_users, users) ->
+  '\x00' :: (app (Proofchat.Pfbytes.int63_to_bytes num_users)
+              (concat (map serialize_username users)))
+| MSG (name, message) ->
+  '\x01' :: (app (serialize_username name) (serialize_string message))
+| ERR err -> '\x02' :: (Proofchat.Pfbytes.int63_to_bytes (int_of_error err))
+
+(** val resend :
+    Uint63.t -> Uint63.t -> Unix.file_descr -> bytes -> Uint63.t -> unit
+    optionE **)
+
+let resend x x0 x1 x2 x3 =
+  let rec hrec fuel n_sent sockfd message len_msg _ =
+    (if sub1_no_underflow fuel
+     then (fun _ ->
+            (let () =
+               print_endline
+                 ((^) "Sent "
+                   ((^)
+                     (string_of_int
+                       (send sockfd message n_sent (sub len_msg n_sent) []))
+                     " bytes"))
+             in
+             (fun _ ->
+             (if ltsb
+                   (add n_sent
+                     (send sockfd message n_sent (sub len_msg n_sent) []))
+                   len_msg
+              then (fun _ ->
+                     hrec (sub fuel (Uint63.of_int (1)))
+                       (add n_sent
+                         (send sockfd message n_sent (sub len_msg n_sent) []))
+                       sockfd message len_msg __)
+              else (fun _ -> SomeE ())) __)) __)
+     else (fun _ -> NoneE
+            ((^) "Timed out while sending message '"
+              ((^) (string_of_bytes message) "'")))) __
+  in hrec x x0 x1 x2 x3 __
+
+(** val send_message : Unix.file_descr -> bytes -> unit optionE **)
+
+let send_message sockfd message =
+  resend (Uint63.of_int (100)) (Uint63.of_int (0)) sockfd message
+    (int_len_list message)
+
+(** val recv_message : Unix.file_descr -> Uint63.t -> bytes **)
+
+let recv_message sockfd len =
+  let (_, out) = recv sockfd (Uint63.of_int (0)) len [] in out
+
+(** val cc_descr :
+    Proofchat.Serverstate.client_connection -> Unix.file_descr **)
+
+let cc_descr = function
+| (_, cc_descr0, _) -> cc_descr0
+
+(** val cc_addr : Proofchat.Serverstate.client_connection -> Unix.sockaddr **)
+
+let cc_addr = function
+| (_, _, cc_addr0) -> cc_addr0
+
+(** val recv_client_message :
+    Proofchat.Serverstate.client_connection -> unit optionE **)
+
+let recv_client_message cc =
+  let () = print_endline "Accepted, can receive!" in
+  let reg_bytes = recv_message (cc_descr cc) (Uint63.of_int (33)) in
+  (match deserialize_client_message reg_bytes with
+   | SomeE x ->
+     (match x with
+      | REG uname ->
+        (match Proofchat.Serverstate.get_connection uname with
+         | Some _ ->
+           let () =
+             print_endline
+               ((^) uname " tried to join, but username already taken")
+           in
+           SomeE ()
+         | None ->
+           let () = print_endline ((^) uname " has joined") in
+           let cc0 = (uname, (cc_descr cc), (cc_addr cc)) in
+           let () = Proofchat.Serverstate.add_connection cc0 in SomeE ())
+      | MESG _ ->
+        send_message (cc_descr cc)
+          (serialize_server_message (ERR UnknownMessageFormat))
+      | PMSG (_, _) ->
+        send_message (cc_descr cc)
+          (serialize_server_message (ERR UnknownMessageFormat))
+      | EXIT _ ->
+        send_message (cc_descr cc)
+          (serialize_server_message (ERR UnknownMessageFormat)))
+   | NoneE _ ->
+     send_message (cc_descr cc)
+       (serialize_server_message (ERR UnknownMessageFormat)))
+
 (** val server_accept_thread : Unix.file_descr -> unit optionE **)
 
 let server_accept_thread socket_fd =
@@ -56,16 +979,19 @@ let server_accept_thread socket_fd =
     let (client_descr, client_addr) = Unix.accept socket_fd in
     let () =
       print_endline
-        ((^) "Accepted client socket "
-          ((^) (string_of_socket_addr client_addr)
-            ((^) " as "
-              (string_of_socket_addr (Unix.getsockname client_descr)))))
+        ((^) "Accepted client socket " (string_of_socket_addr client_addr))
     in
-    NoneE "server_accept_thread recurse")
+    let () =
+      keep
+        (Thread.create recv_client_message (dummy_username, client_descr,
+          client_addr))
+    in
+    Recurse)
 
 (** val server : string -> int -> unit optionE **)
 
 let server host portno =
+  let () = Proofchat.Serverstate.init_connections () in
   let socket_fd =
     Unix.socket Unix.PF_INET Unix.SOCK_STREAM (Uint63.of_int (0))
   in
