proofchat/bin/server/server.mli
@@ -1,5 +1,56 @@
 
+type nat =
+| O
+| S of nat
+
+val app : 'a1 list -> 'a1 list -> 'a1 list
+
+type positive =
+| XI of positive
+| XO of positive
+| XH
+
+type n =
+| N0
+| Npos of positive
+
+module Pos :
+ sig
+  val succ : positive -> positive
+
+  val of_succ_nat : nat -> positive
+ end
+
+module N :
+ sig
+  val of_nat : nat -> n
+ end
+
+val zero : char
+
+val one : char
+
+val shift : bool -> char -> char
+
+val ascii_of_pos : positive -> char
+
+val ascii_of_N : n -> char
+
+val ascii_of_nat : nat -> char
+
+
+
+val rev : 'a1 list -> 'a1 list
+
+val concat : 'a1 list list -> 'a1 list
+
+val map : ('a1 -> 'a2) -> 'a1 list -> 'a2 list
+
+val add : Uint63.t -> Uint63.t -> Uint63.t
+
 val sub : Uint63.t -> Uint63.t -> Uint63.t
+
+val eqb : Uint63.t -> Uint63.t -> bool
 
 val ltsb : Uint63.t -> Uint63.t -> bool
 
@@ -11,11 +62,102 @@ type 'x optionE =
 | SomeE of 'x
 | NoneE of string
 
+type bytes = char list
+
+val send :
+  Unix.file_descr -> bytes -> Uint63.t -> Uint63.t -> Unix.msg_flag list ->
+  Uint63.t
+
+val recv :
+  Unix.file_descr -> Uint63.t -> Uint63.t -> Unix.msg_flag list ->
+  Uint63.t * bytes
+
+val keep : 'a1 -> unit
+
 val sub1_no_underflow : Uint63.t -> bool
 
-val repeat_until_timeout : Uint63.t -> (unit -> unit optionE) -> unit optionE
+type repeat_until_timeout_code =
+| Recurse
+| EarlyStopSuccess
+| EarlyStopFailure of string
+
+val repeat_until_timeout :
+  Uint63.t -> (unit -> repeat_until_timeout_code) -> unit optionE
+
+val space : char
+
+val no_spaces : string -> bool
 
 val string_of_socket_addr : Unix.sockaddr -> string
+
+val int_len_list : 'a1 list -> Uint63.t
+
+val bytes_of_string : string -> bytes
+
+val string_of_bytes : bytes -> string
+
+val int_len_string : string -> Uint63.t
+
+val create_list : 'a1 -> Uint63.t -> 'a1 list
+
+val pad_string_r : string -> char -> Uint63.t -> string
+
+val first_n : 'a1 list -> Uint63.t -> 'a1 list optionE
+
+val last_n : 'a1 list -> Uint63.t -> 'a1 list optionE
+
+type username =
+  string
+  (* singleton inductive, whose constructor was Build_username *)
+
+val validate_username : string -> bool
+
+val new_username : string -> username optionE
+
+val dummy_username : username
+
+val serialize_string : string -> bytes
+
+val serialize_username : username -> bytes
+
+type client_message =
+| REG of username
+| MESG of string
+| PMSG of string * username
+| EXIT of username
+
+val deserialize_client_message : bytes -> client_message optionE
+
+type error =
+| UsernameTaken
+| UsernameTooLong
+| UsernameHasSpaces
+| PmsgTargetNotExists
+| UnknownMessageFormat
+| Error
+
+val int_of_error : error -> Uint63.t
+
+type server_message =
+| ACK of Uint63.t * username list
+| MSG of username * string
+| ERR of error
+
+val serialize_server_message : server_message -> bytes
+
+val resend :
+  Uint63.t -> Uint63.t -> Unix.file_descr -> bytes -> Uint63.t -> unit optionE
+
+val send_message : Unix.file_descr -> bytes -> unit optionE
+
+val recv_message : Unix.file_descr -> Uint63.t -> bytes
+
+val cc_descr : Proofchat.Serverstate.client_connection -> Unix.file_descr
+
+val cc_addr : Proofchat.Serverstate.client_connection -> Unix.sockaddr
+
+val recv_client_message :
+  Proofchat.Serverstate.client_connection -> unit optionE
 
 val server_accept_thread : Unix.file_descr -> unit optionE
 
