proofchat/lib/pfbytes.ml
@@ -1,8 +1,23 @@
-let bytes_of_byte_list (l : char list) : bytes =
+open Unix
+
+let bytes_of_char_list (l : char list) : bytes =
   Bytes.concat Bytes.empty (List.map (fun c -> Bytes.make 1 c) l)
 
-let int63_to_bytes n =
+let char_list_of_bytes (b : bytes) : char list =
+  let l = ref [] in
+  for i = 0 to Bytes.length b - 1 do
+    l := Bytes.get b i :: !l
+  done;
+  List.rev !l
+
+let int63_to_bytes (n : int) : char list =
   List.map (fun i -> Char.chr ((n lsr (i * 8)) land 0xFF)) [0;1;2;3;4;5;6;7]
 
-let bytes_to_int63 bytes =
-  List.fold_left (fun a b -> a + (int_of_char b)) 0 bytes
+let bytes_to_int63 (b : char list) : int =
+  List.fold_left (fun a b -> a + (int_of_char b)) 0 b
+
+let functional_read (fd : file_descr) (pos : int) (len : int) (flags : msg_flag list) 
+    : int * char list =
+  let b = Bytes.create len in
+  let num_read = recv fd b pos len flags in
+  (num_read, char_list_of_bytes b)
