proofchat/lib/serverstate.ml
@@ -1,0 +1,37 @@
+open Unix
+
+type client_connection = string * file_descr * sockaddr 
+(* {
+    cc_uname : string
+  ; cc_descr : file_descr
+  ; cc_addr : sockaddr
+} *)
+
+let atom (f : unit -> 'a) : 'a =
+  let m = Mutex.create () in
+  Mutex.lock m;
+  try
+    f ()
+  with e ->
+    Mutex.unlock m;
+    raise e
+
+let connections : (client_connection list) ref = 
+  ref []
+
+let init_connections () =
+  atom (fun _ -> connections := [])
+
+let add_connection (c : client_connection) =
+  atom (fun _ -> connections := (c :: !connections))
+
+let remove_connection (c : client_connection) =
+  atom (fun _ -> 
+    connections := List.filter (fun c' -> c' != c) !connections)
+
+let get_connection (s : string) : client_connection option =
+  atom (fun _ -> 
+    match (List.filter 
+      (function (cc_uname, _, _) -> cc_uname = s) !connections) with
+    | h :: _ -> Some h
+    | _ -> None)
