theories/PCExtract.v
@@ -8,7 +8,7 @@ Require Import StringTheory.
 Require Import Client.
 Require Import Server.
 Require Import Monads.
-Require Import Sockets.
+Require Import Unix.
 Require Import ExtrOcamlBasic.
 Require Import ExtrOcamlNativeString.
 Require Import ExtrOCamlInt63.
@@ -16,9 +16,11 @@ Require Import ExtrOCamlInt63.
 Extraction Language OCaml.
 Unset Extraction Optimize.
 
+(** ** Functions *)
 Extract Inlined Constant read_line => "read_line".
 Extract Inlined Constant print_int => "print_int".
 Extract Inlined Constant print_string => "print_string".
+Extract Constant print_bytes => "(fun b -> print_bytes (Proofchat.Pfbytes.bytes_of_char_list b))".
 Extract Inlined Constant print_endline => "print_endline".
 Extract Inlined Constant string_of_int => "string_of_int".
 Extract Inlined Constant socket => "Unix.socket".
@@ -32,11 +34,23 @@ Extract Inlined Constant connect => "Unix.connect".
 Extract Inlined Constant accept => "Unix.accept".
 Extract Inlined Constant bind => "Unix.bind".
 Extract Inlined Constant listen => "Unix.listen".
-Extract Constant send => "(fun a b c d e -> Unix.send a (Proofchat.Pfbytes.bytes_of_byte_list b) c d e)".
+Extract Constant send => "(fun a b c d e -> Unix.send a (Proofchat.Pfbytes.bytes_of_char_list b) c d e)".
+Extract Constant recv => "Proofchat.Pfbytes.functional_read".
 Extract Inlined Constant close => "Unix.close".
 Extract Inlined Constant int63_to_bytes => "Proofchat.Pfbytes.int63_to_bytes".
 Extract Inlined Constant bytes_to_int63 => "Proofchat.Pfbytes.bytes_to_int63".
+Extract Inlined Constant create => "Thread.create".
+Extract Inlined Constant join => "Thread.join".
+Extract Inlined Constant exit => "Thread.exit".
+Extract Constant keep => "(fun _ -> ())".
 
+(** ** Server state *)
+Extract Inlined Constant init_connections => "Proofchat.Serverstate.init_connections".
+Extract Inlined Constant add_connection => "Proofchat.Serverstate.add_connection".
+Extract Inlined Constant remove_connection => "Proofchat.Serverstate.remove_connection".
+Extract Inlined Constant get_connection => "Proofchat.Serverstate.get_connection".
+
+(** ** Types *)
 Extract Inlined Constant port => "int".
 Extract Inductive socket_domain => 
     "Unix.socket_domain" [ "Unix.PF_UNIX" "Unix.PF_INET" "Unix.PF_INET6" ].
@@ -46,7 +60,15 @@ Extract Inductive sockaddr =>
     "Unix.sockaddr" [ "Unix.ADDR_UNIX" "Unix.ADDR_INET" ].
 Extract Inductive msg_flag =>
     "Unix.msg_flag" [ "Unix.MSG_OOB" "Unix.MSG_DONTROUTE" "Unix.MSG_PEEK" ].
+Extract Inlined Constant inet_addr => "Unix.inet_addr".
+Extract Inlined Constant file_descr => "Unix.file_descr".
+Extract Inlined Constant thread => "Thread.t".
+Extract Inductive client_connection =>
+    "Proofchat.Serverstate.client_connection" 
+    [ "" ].
+(* Extract Inlined Constant cc_uname => "(fun x -> x.cc_uname)". *)
 
+(** ** Extraction *)
 Set Extraction Output Directory "proofchat/bin/client".
 Recursive Extraction client.
 Extraction "client.ml" client.
