theories/Server.v
@@ -1,5 +1,5 @@
 (** * Server
-    
+
     In this section, we define program logic for the host server
 *)
 
@@ -8,6 +8,56 @@ Require Import Monads.
 Require Import Recdef.
 Open Scope monad_scope.
 
+
+(** ** Server state 
+
+    In this section, we define types and axioms to bind to the
+    Proofchat.Serverstate module that handles CRUD operations for the server
+    in a thread-safe manner using mutexes.
+*)
+Record client_connection : Type := {
+      cc_uname : username
+    ; cc_descr : file_descr
+    ; cc_addr : sockaddr
+}.
+Axiom init_connections : unit -> unit.
+Axiom add_connection : client_connection -> unit.
+Axiom remove_connection : client_connection -> unit.
+Axiom get_connection : username -> option client_connection.
+
+Definition recv_client_message (cc : client_connection) : optionE unit :=
+    let* _ <= print_endline "Accepted, can receive!" #;
+    (* Read 33 bytes - should be a REG message *)
+    let reg_bytes := recv_message cc.(cc_descr) 33 in
+    match (deserialize_client_message reg_bytes) with
+    | SomeE (REG uname) =>
+        match get_connection uname with
+        (* Username is not taken *)
+        | None => 
+            (* Add the new connection *)
+            let* _ <= print_endline (uname.(Uname) ++ " has joined") #;
+            let cc := {|
+                cc_uname := uname; 
+                cc_descr := cc.(cc_descr); 
+                cc_addr := cc.(cc_addr)
+            |} in
+            let* _ <= add_connection cc #;
+            (* temporary *)
+            (* let* _ <= remove_connection cc #; *)
+            return tt
+        (* Username is taken *)
+        | Some _ =>
+            let* _ <= print_endline (uname.(Uname) ++ 
+                " tried to join, but username already taken") #;
+            (* _ <- send_message cc.(cc_descr)
+                (serialize_server_message (ERR UsernameTaken)) ;; *)
+            return tt
+        end
+    | _ => 
+        send_message cc.(cc_descr)
+            (serialize_server_message (ERR UnknownMessageFormat))
+    end.
+
 (**
     Accept new connections and spawn synchronization threads for each of them
 *)
@@ -15,15 +65,17 @@ Definition server_accept_thread (socket_fd : file_descr) : optionE unit :=
     repeat_until_timeout max_int (fun _ =>
         let '(client_descr, client_addr) := accept socket_fd in
         let* _ <= print_endline 
-            ("Accepted client socket " ++ (string_of_socket_addr client_addr)
-             ++ " as " ++ (string_of_socket_addr (getsockname client_descr))) #;
-        NoneE "server_accept_thread recurse"
+            ("Accepted client socket " ++ (string_of_socket_addr client_addr)) #;
+        let* _ <= keep thread (create client_connection (optionE unit) recv_client_message
+            {|cc_uname := dummy_username; cc_descr := client_descr; cc_addr := client_addr|}) #;
+        Recurse
     ).
 
 (**
     Wraps up all server logic: port binding, threading, etc.
 *)
 Definition server (host : string) (portno : port) : optionE unit :=
+    let* _ <= init_connections tt #;
     (* Create a TCP socket *)
     let socket_fd := socket PF_INET SOCK_STREAM 0 in
     let socket_addr := ADDR_INET (inet_addr_of_string host) portno in
@@ -35,10 +87,6 @@ Definition server (host : string) (portno : port) : optionE unit :=
     let* _ <= listen socket_fd 10 #;
     let* _ <= print_endline "Server started" #;
     _ <- server_accept_thread socket_fd ;;
-    (* Receive ACK from server *)
-    (* Display chatroom information to user output *)
-    (* Wait for user input *)
-    (* Wait for chat messages from server *)
     let* _ <= print_endline "Closing server" #;
     let* _ <= close socket_fd #;
     return tt.
