make_docs.sh
@@ -1,5 +1,2 @@
-rm -r docs
 make html
-mv html docs
-echo "This entire folder is deleted and auto-generated via `make html`" > docs/WARNING
-rm -r html
+mv html/* docs/ && rm -r html
